intermediate/Veritas.Intermediate.VerifyS.fsti
@@ -277,180 +277,6 @@ let vevictbm (s:slot_id) (s':slot_id) (t:timestamp) (vs:vtls {Valid? vs}): vtls 
           else
             let st_upd = update_hash_and_blum_bit st s' d h2 true in
             vevictb s t (update_thread_store vs st_upd)
-
-(* Relation between SC and S thread-local states *)
-  
-let vtls_rel (vs:vtls) (vs':SC.vtls) : Type =
-  (Failed? vs /\ SC.Failed? vs') \/
-  (Valid? vs /\ SC.Valid? vs' /\
-   (let (Valid id st clk ha he) = vs in
-    let (SC.Valid id' st' clk' ha' he') = vs' in
-    // all fields are equal
-    equal_contents st st' /\ id = id' /\ clk = clk' /\ ha = ha' /\ he = he' /\
-    // the invariant over MAdd keys holds
-    merkle_store_inv st))
-
-let lemma_vget_simulates_SC 
-      (vs:vtls{Valid? vs})
-      (vs':SC.vtls{SC.Valid? vs'})
-      (s:slot_id)
-      (k:data_key)
-      (v:data_value)
-  : Lemma (requires (vtls_rel vs vs'))
-          (ensures (vtls_rel (vget s k v vs) (SC.vget s k v vs')))
-  = ()
-
-let lemma_update_value_DVal_preserves_merkle_inv (st:vstore) (s:slot_id{store_contains st s /\ is_data_key (stored_key st s)}) (v:data_value)
-  : Lemma (requires merkle_store_inv st)
-          (ensures merkle_store_inv (update_value st s (DVal v)))
-          [SMTPat (merkle_store_inv (update_value st s (DVal v)))]
-  = admit()
-
-let lemma_vput_simulates_SC
-      (vs:vtls{Valid? vs}) 
-      (vs':SC.vtls{SC.Valid? vs'}) 
-      (s:slot_id) 
-      (k:data_key) 
-      (v:data_value) 
-  : Lemma (requires (vtls_rel vs vs'))
-          (ensures (vtls_rel (vput s k v vs) (SC.vput s k v vs'))) 
-  = ()
-
-#push-options "--z3rlimit_factor 2"
-let lemma_vaddm_simulates_SC 
-      (vs:vtls{Valid? vs}) 
-      (vs':SC.vtls{SC.Valid? vs'}) 
-      (s s':slot_id)
-      (r:record)  
-  : Lemma (requires (vtls_rel vs vs'))
-          (ensures (vtls_rel (vaddm s r s' vs) (SC.vaddm s r s' vs'))) 
-  = if s < thread_store_size vs
-    then 
-      let st = thread_store vs in
-      let (k,v) = r in
-      if store_contains st s'
-      then
-        let k' = stored_key st s' in
-        let v' = stored_value st s' in
-        if is_proper_desc k k' && not (store_contains st s) && is_value_of k v && not (DVal? v')
-        then
-          let v' = to_merkle_value v' in
-          let d = desc_dir k k' in
-          let dh' = desc_hash_dir v' d in 
-          let h = hashfn v in
-          let st' = SC.thread_store vs' in
-          match dh' with
-          | Empty -> 
-              // CASE 1 - by points_to_nearest_desc_in_store, either k is not in the store or 
-              //          the final hash check is guaranteed to fail
-              assert (points_to_nearest_desc_in_store st s');
-              if v = init_value k 
-              then (
-                let v'_upd = Spec.update_merkle_value v' d k h false in
-                let st_upd = update_value st s' (MVal v'_upd) in
-                let st_upd2 = add_to_store st_upd s k v Spec.MAdd in
-                let st_upd3 = update_in_store st_upd2 s' d true in
-                assume (merkle_store_inv st_upd3)
-              )
-          | Desc k2 h2 b2 -> 
-              if k2 = k 
-              // CASE 2 - by in_store_flag_implies.. and evicted_to_blum_flag_implies.., either 
-              //          k is not in the store or the final hash check is guaranteed to fail
-              then (
-                assert (in_store_flag_unset_equals_desc_not_in_store st s');              
-                if h2 = h && b2 = false
-                then 
-                if not (child_in_store st s' d)
-                then (
-                  assert (not (store_contains_key_with_MAdd st k));
-                  let st_upd = add_to_store st s k v Spec.MAdd in
-                  let st_upd2 = update_in_store st_upd s' d true in
-                  assume (merkle_store_inv st_upd2)
-                )
-              )
-              // CASE 3 - similar to CASE 1
-              else (
-                assert (points_to_nearest_desc_in_store st s');              
-                if v = init_value k && is_proper_desc k2 k 
-                then
-                  let d2 = desc_dir k2 k in
-                  let mv = to_merkle_value v in
-                  let mv_upd = Spec.update_merkle_value mv d2 k2 h2 b2 in
-                  let v'_upd = Spec.update_merkle_value v' d k h false in
-                  let st_upd = update_value st s' (MVal v'_upd) in
-                  let st_upd2 = add_to_store st_upd s k (MVal mv_upd) Spec.MAdd in
-                  let st_upd3 = update_in_store st_upd2 s' d true in
-                  let st_upd4 = update_in_store st_upd3 s d2 true in
-                  assume (merkle_store_inv st_upd4)
-              )
-#pop-options
-
-let lemma_evict_from_store_preserves_inv (st:vstore) (s:slot_id{store_contains st s})
-  : Lemma (requires merkle_store_inv st)
-          (ensures merkle_store_inv (evict_from_store st s))
-          [SMTPat (merkle_store_inv (evict_from_store st s))]
-  = admit()
-
-let lemma_has_in_store_merkle_desc (st:vstore) (st':SCstore.vstore) (s:slot_id{store_contains st s})
-  : Lemma (requires equal_contents st st' /\ merkle_store_inv st)
-          (ensures has_instore_merkle_desc st s = SC.has_instore_merkle_desc st' (SCstore.stored_key st' s))
-          [SMTPat (has_instore_merkle_desc st s); SMTPat (SC.has_instore_merkle_desc st' (SCstore.stored_key st' s))]
-  = admit()
-
-let lemma_update_hash_and_blum_bit_preserves_inv 
-      (st:vstore) 
-      (s:slot_id{store_contains st s /\ MVal? (stored_value st s)}) 
-      (d:bin_tree_dir{Desc? (desc_hash_dir (to_merkle_value (stored_value st s)) d)}) 
-      (h:hash_value)
-      (b:bool)
-  : Lemma (requires merkle_store_inv st)
-          (ensures merkle_store_inv (update_hash_and_blum_bit st s d h b)) 
-          [SMTPat (merkle_store_inv (update_hash_and_blum_bit st s d h b))]
-  = admit()
-
-let lemma_vevictm_simulates_SC 
-      (vs:vtls{Valid? vs}) 
-      (vs':SC.vtls{SC.Valid? vs'}) 
-      (s s':slot_id)  
-  : Lemma (requires (vtls_rel vs vs'))
-          (ensures (vtls_rel (vevictm s s' vs) (SC.vevictm s s' vs'))) 
-  = ()
-
-let lemma_add_to_store_BAdd_preserves_inv (st:vstore) (s:st_index st{not (store_contains st s)}) (k:key) (v:value_type_of k)
-  : Lemma (requires merkle_store_inv st)
-          (ensures merkle_store_inv (add_to_store st s k v Spec.BAdd))
-          [SMTPat (merkle_store_inv (add_to_store st s k v Spec.BAdd))]
-  = admit()
-
-let lemma_vaddb_simulates_SC 
-      (vs:vtls{Valid? vs}) 
-      (vs':SC.vtls{SC.Valid? vs'}) 
-      (s:slot_id)
-      (r:record)
-      (t:timestamp)
-      (j:thread_id)
-  : Lemma (requires (vtls_rel vs vs'))
-          (ensures (vtls_rel (vaddb s r t j vs) (SC.vaddb s r t j vs')))
-  = ()
-
-let lemma_vevictb_simulates_SC 
-      (vs:vtls{Valid? vs}) 
-      (vs':SC.vtls{SC.Valid? vs'}) 
-      (s:slot_id)
-      (t:timestamp)
-  : Lemma (requires (vtls_rel vs vs'))
-          (ensures (vtls_rel (vevictb s t vs) (SC.vevictb s t vs'))) 
-          [SMTPat (vtls_rel (vevictb s t vs) (SC.vevictb s t vs'))]
-  = ()
-
-let lemma_vevictbm_simulates_SC 
-      (vs:vtls{Valid? vs}) 
-      (vs':SC.vtls{SC.Valid? vs'}) 
-      (s s':slot_id)
-      (t:timestamp)
-  : Lemma (requires (vtls_rel vs vs'))
-          (ensures (vtls_rel (vevictbm s s' t vs) (SC.vevictbm s s' t vs'))) 
-  = ()
   
 let t_verify_step (vs:vtls) (e:logS_entry): vtls =
   match vs with
@@ -491,9 +317,21 @@ let init_thread_state (id:thread_id): vtls =
 let t_verify (id:thread_id) (l:logS): vtls = 
   t_verify_aux (init_thread_state id) l 
 
-val init_thread_state_valid (id:thread_id)
+(* Relation between SC and S thread-local states *)
+let vtls_rel (vs:vtls) (vs':SC.vtls) : Type =
+  (Failed? vs /\ SC.Failed? vs') \/
+  (Valid? vs /\ SC.Valid? vs' /\
+   (let (Valid id st clk ha he) = vs in
+    let (SC.Valid id' st' clk' ha' he') = vs' in
+    // all fields are equal
+    equal_contents st st' /\ id = id' /\ clk = clk' /\ ha = ha' /\ he = he' /\
+    // the invariant over MAdd keys holds
+    merkle_store_inv st))
+
+let init_thread_state_valid (id:thread_id)
   : Lemma (Valid? (init_thread_state id))
           [SMTPat (init_thread_state id)]
+  = ()
 
 val lemma_init_thread_state_rel (id:thread_id)
   : Lemma (vtls_rel (init_thread_state id) (SC.init_thread_state id))
@@ -510,25 +348,64 @@ let verifiable (gl: g_logS) =
 
 let verifiable_log = gl:g_logS{verifiable gl}
 
-val hadd (gl: verifiable_log): ms_hash_value
+val lemma_prefix_verifiable (gl: verifiable_log) (i:seq_index gl)
+  : Lemma (ensures verifiable (prefix gl i))
+          [SMTPat (verifiable (prefix gl i))]
 
-val hevict (gl: verifiable_log): ms_hash_value
+let rec hadd_aux (gl: verifiable_log)
+  : Tot (ms_hash_value)
+    (decreases (Seq.length gl)) 
+  = let p = Seq.length gl in
+    if p = 0 then empty_hash_value
+    else
+      let gl' = prefix gl (p - 1) in
+      let h1 = hadd_aux gl' in
+      let h2 = thread_hadd (verify (thread_log gl (p - 1))) in
+      ms_hashfn_agg h1 h2
 
-let hash_verifiable (gl: verifiable_log): bool = 
-  hadd gl = hevict gl
+let hadd (gl: verifiable_log): ms_hash_value = hadd_aux gl
+
+let rec hevict_aux (gl: verifiable_log)
+  : Tot (ms_hash_value)
+    (decreases (Seq.length gl))
+  = let p = Seq.length gl in
+    if p = 0 then empty_hash_value
+    else
+      let gl' = prefix gl (p - 1) in
+      let h1 = hevict_aux gl' in
+      let h2 = thread_hevict (verify (thread_log gl (p - 1))) in
+      ms_hashfn_agg h1 h2
+
+let hevict (gl: verifiable_log): ms_hash_value = hevict_aux gl
+
+let hash_verifiable (gl: verifiable_log): bool
+  = hadd gl = hevict gl
 
 let hash_verifiable_log = gl:verifiable_log{hash_verifiable gl}
 
 let lemma_verifiable_simulates_SC (gl:verifiable_log)
   : Lemma (ensures SC.verifiable gl)
           [SMTPat (SC.verifiable gl)]
+  = let aux (tid:seq_index gl) : Lemma (SC.Valid? (SC.verify (thread_log gl tid)))
+      = lemma_t_verify_simulates_SC tid (Seq.index gl tid) in
+    Classical.forall_intro aux
+
+val hadd_values_equal (gl:verifiable_log) : Lemma (hadd gl = SC.hadd gl)
+
+val hevict_values_equal (gl:verifiable_log) : Lemma (hevict gl = SC.hevict gl)
+
+(* We show in VerifySC.fst that forall_is_map gl <==> forall i. thread_store_is_map (verify (thread_log gl i)).
+   So the easiest way to prove this lemma is probably by showing that if there is any case where is_map becomes false
+   (only possible in SCstore.add_to_store), then the final hash check must fail. *)
+let lemma_hash_verifiable_log_implies_forall_is_map (gl:hash_verifiable_log)
+  : Lemma (SC.forall_is_map gl)
   = admit()
 
 let lemma_hash_verifiable_simulates_SC (gl:hash_verifiable_log)
   : Lemma (SC.hash_verifiable gl)
-  = admit() 
-    // requires showing that hash check succeeds ==> SC returns is_map=true for every thread
-    // alternatively, if SC returns is_map=false for any thread, then the hash check will fail
+  = hadd_values_equal gl;
+    hevict_values_equal gl;
+    lemma_hash_verifiable_log_implies_forall_is_map gl 
 
 (* Correctness *)
 
